WIP on forcing values to have valid denotations

coq/denot/definitions.v
@@ -14,7 +14,7 @@
    the set is the complete denotation of the value/computation. (These
    elements should be consistent with eachother.)
 
-   The denotation of both values and computations includes bottom: the
+   The denotation of both values and computations includes the empty set: the
    denotation of an infinite loop. Therefore, some definitions include
    the predicate
 
@@ -30,14 +30,16 @@
    computations.
 
    However, I was unable to prove continuity for the semantic operators using
-   this definition. So I have used the types above, and have defined the
+   this definition. 
+
+   So I have used the types above, and have defined the
    Monad-like operations:
 
       RET : P A -> P (Comp (list A))
 
       BIND : (P (Comp (list A))) -> (P A -> P (Comp B)) -> P (Comp B)
 
-   I don't know which of the analogous monad laws these operators satisfy.
+   I don't know which of the analogous monad laws these operators satisfy. 
 
    Other semantic operators:
 
@@ -51,9 +53,13 @@
 
       LIST : list (P Value) -> P Value
 
-      Λ : (P Value -> P (Comp (list Value))) -> P Value     -- note function bodies are computations
+      Λ : (P Value -> P (Comp (list Value))) -> P Value     
+             -- note function bodies are computations, so functions can 
+             -- produce errors or multiple results
 
       APPLY : P Value -> P Value -> P (Comp (list Value))
+             -- application requires two (valid) values because we can use 
+             -- BIND above to sequence the computations first
 
    Environments. An `Env A` is an association list, associating each variable with an `A`. 
 
@@ -89,31 +95,55 @@ Require Import Lia.
 
 Require Export lc.tactics.
 Require Import structures.Structures.
+Require Import semantic_notions.
+Require Import QuasiMonad.
 
 Import MonadNotation.
 Open Scope monad_scope.
 Import SetNotations.
 Local Open Scope set_scope.
 
-(* Sets of Values:   P Value === Value -> Prop *)
 
-(* ------------------------------------------------------- *)
+(*
+Definition PP (A : Type) : Type := { V : P A |  nonempty V}.
 
-(* `P (Comp (P A))` is *almost* a Monad *)
+Definition PP_Singleton {A : Type} (x : A) : PP A := 
+  exist (fun V : P A => nonempty V) ⌈ x ⌉ (Inhabited_intro A ⌈ x ⌉ x in_singleton).
 
-Definition RET {A} (x : P A) : P (Comp (list A)) :=
-  fun z => match z with 
-          | c_multi (V :: nil) => (mem V ⊆ x) /\ V <> nil
-          |  _ => False
-        end.
+Definition PP_In {A : Type} (s : PP A) (x : A) : Prop.
+destruct s as [x0 _]. exact (x0 x). Defined.
 
-(* V must be nonempty because RET is strict. If V is empty then the 
-   set should be empty. *)
+Definition PP_Included {A : Type} (x : PP A) (y : PP A) : Prop := forall z, PP_In x z -> PP_In y z.
 
-Definition BIND {A B} (S : P (Comp (list A))) (K : P A -> P (Comp B)) (t : Comp B) : Prop :=
-  exists (u : Comp (list A)), exists (k : list A -> Comp B), 
-    S u /\ t = bind u k /\ forall a, Comp_In a u -> K (mem a) (k a).
+Definition PP_Union {A : Type} (x : PP A) (y : PP A) : PP A.
+  destruct x. destruct y. exists (Union x x0). 
+  destruct n. destruct n0.
+  eapply Inhabited_intro with (x := x1).
+  econstructor. exact H.
+Defined.
 
+Definition PP_Same_set {A : Type} (x : PP A) (y : PP A) : Prop.
+  destruct x as [s _]. destruct y as [t _]. 
+  exact (Same_set s t). 
+Defined.
+  
+Declare Scope pset_scope.
+Delimit Scope pset_scope with PP.
+Bind Scope pset_scope with PP.
+
+Module PSetNotations. 
+  Notation "x ∈ s" := (PP_In s x) : pset_scope .
+  Notation "⌈ x ⌉" := (PP_Singleton x) : pset_scope.
+  Infix "⊆" := PP_Included : pset_scope.
+  Infix "∪" := PP_Union : pset_scope.
+  Infix "≃" := PP_Same_set : pset_scope.
+End PSetNotations.
+
+Import PSetNotations.
+Open Scope pset_scope.
+
+*)
+  
 (* ----------------------------------------------------------- *)
 
 Inductive Value : Type :=
@@ -121,7 +151,7 @@ Inductive Value : Type :=
   | v_nat : nat -> Value
 
   (* one entry in a function's table *)
-  | v_map : list Value -> Comp (list Value) -> Value
+  | v_map : forall (x: list Value), Comp Value -> Value
 
   (* trivial function value, evaluated to a value but never applied *)
   | v_fun : Value
@@ -144,22 +174,6 @@ Denotation of Identity function (\x.x):
 
 Infix "↦" := v_map (at level 85, right associativity).
 
-(* ------------ Valid values and computations ------------------ *)
-
-
-Definition valid (V : P Value) : Type :=
-  nonemptyT V.
-
-Definition valid_mem (V : list Value) : Prop :=
-  V <> nil.
-
-(* Produces at least one result *)
-
-(*
-Definition valid_Comp (C : P (Comp Value)) : Type :=
-  (nonemptyT C * not (c_wrong ∈ C) * not (c_multi nil ∈ C))%type.
-*)
-
 (* ------------ Semantic Operators ------------------ *)
 
 Definition NAT : nat -> P Value :=
@@ -180,17 +194,72 @@ Definition NIL : P Value := ⌈ v_list nil ⌉.
 Definition CONS : P Value -> P Value -> P Value := 
   fun V W x => 
     match x with 
-    | v_list (v :: w) => (v ∈ V) /\ (v_list w ∈ W)  (* v should not be wrong *)
+    | v_list (v :: w) => (v ∈ V) /\ (v_list w ∈ W)  
     | _ => False
     end.
 
-Definition Λ : (P Value -> P (Comp (list Value))) -> P Value :=
+Definition coerce (w : Comp Value) : Comp (vfin Value) := 
+  fmap (fun x => 
+  match w with 
+  | c_wrong => X c_wrong
+  | c_multi lw => 
+      match c with 
+    | c_wrong => False
+    | c_multi l => List.Forall2 (fun v vf => v ∈ vmem vf) w l
+    end.
+
+Definition Λ : (P Value -> P (Comp (vfin Value))) -> P Value :=
   fun f => fun v => match v with 
           | (V ↦ w) => (w ∈ (f (mem V))) /\ valid_mem V  (* CBV *)
           | v_fun => True
           | _ => False
           end.
 
+
+(* ------------ LOGIC PROGRAMMING ----------------- *)
+
+Definition ONE (C : P (Comp (list Value))) : P Value :=
+  fun v => exists l, c_multi (ret v  :: l) ∈ C.
+
+Definition ALL (C : P (Comp (list Value))) : P Value :=
+  fun v => match v with 
+          | v_list l => c_multi (List.map ret l) ∈ C 
+          | _ => False
+        end.
+
+Definition FAIL : P (Comp (list Value)) := ⌈ c_multi nil ⌉.
+
+Definition CHOOSE (C1 : P (Comp (list Value))) (C2 : P (Comp (list Value))) : 
+  P (Comp (list Value)) := 
+  fun c => 
+    match c with 
+    | c_multi l => 
+        exists l1, exists l2, l = l1 ++ l2 /\ (c_multi l1 ∈ C1) /\ (c_multi l2 ∈ C2)
+    | _ => False
+    end.
+
+(* Fails when V and W don't unify. Returns their union when they do. *)
+(* Need to define inconsistent here.
+
+Definition UNIFY (V : P Value) (W: P Value) : P (Comp (list Value)) :=
+  fun c => match c with 
+
+        | c_multi nil => 
+            exists v, exists w, v ∈ V /\ w ∈ W /\ Inconsistent v w
+
+        | c_multi (l :: nil) => (mem l ⊆ V ∪ W) /\ l <> nil
+
+        | _ => False
+  end.
+*)    
+  
+
+(* ------------------------------------------ *)
+
+(* This definition includes all values that produce c. *)
+
+Definition EXISTS (f : P Value -> P (Comp (list Value))) : P (Comp (list Value)) :=
+  fun c => exists V, c ∈ f (mem V).
 
 (* ------------ APPLY ----------------- *)
 
