coq/denot/QuasiMonad.v
@@ -1,0 +1,516 @@
+Require Import Coq.Logic.FunctionalExtensionality.
+Require Import Coq.Classes.RelationClasses.
+Require Coq.Relations.Relation_Definitions.
+Require Import Lia.
+
+Require Export lc.tactics.
+Require Import structures.Structures.
+Require Import denot.semantic_notions. 
+
+Import MonadNotation.
+Open Scope monad_scope.
+Import SetNotations.
+Local Open Scope set_scope.
+
+(* ------------------------------------------------------- *)
+
+Definition RET {A} (x : P A) : P (Comp (vfin A)) :=
+  fun z => match z with 
+          | c_multi (V :: nil) => (vmem V ⊆ x)   
+          |  _ => False
+        end.
+
+(* Q: can we get rid of V <> nil ? What part of the proof breaks? *)
+
+(* A: V must be nonempty because RET is strict. If x is ⊥ then the 
+   returned Comp set should be ⊥ not c_multi [ ⊥ ] . 
+
+   A: But, really RET should only be applied to nonempty x. Maybe 
+   we shouldn't care about what happens when x is ⊥ ?
+
+*)
+
+
+Definition BIND {A B} (S : P (Comp (vfin A))) (K : P A -> P (Comp B)) : P (Comp B) :=
+  fun t => 
+   exists (s : Comp (vfin A)),    (* in S *)
+   exists (k : vfin A -> Comp B),  (* in K, for every valid finite set in u *)
+       t = bind s k          (* produces t *)
+      /\ (s ∈ S)      
+      /\ forall (V : vfin A),
+          Comp_In V s -> (k V) ∈ K (vmem V).    
+
+(* Above, we need V nonempty to show that m ⊆ BIND m RET  as RET is strict *)
+
+(* ------------------------------------------------------- *)
+
+Lemma RET_mono {A} : forall (U V : P A), 
+ U ⊆ V -> RET U ⊆ RET V. 
+Proof. 
+    intros U V h x xIn.
+    unfold Included in h.
+    destruct x; simpl in *; eauto.
+    destruct l as [| y t]; try done.
+    destruct t; try done.
+    unfold RET in *. cbn in *.
+    unfold Included in xIn.
+    intros x. 
+    eauto.
+Qed.
+
+Lemma RET_cong {A} : forall (U V : P A), 
+ U ≃ V -> RET U ≃ RET V. 
+Proof. 
+intros x1 y1 E1. split. eapply RET_mono. rewrite E1. reflexivity.
+eapply  RET_mono. rewrite E1. reflexivity.
+Qed.
+
+#[export] Instance Proper_Included_RET {A} : Proper (Included ==> Included) 
+                                               (@RET A).
+unfold Proper. intros x1 y1 E1. eapply RET_mono; auto. Qed.
+
+#[export] Instance Proper_Same_RET {A} : Proper (Same_set ==> Same_set) (@RET A).
+unfold Proper. intros x1 y1 E1. eapply RET_cong; auto. Qed.
+
+Lemma BIND_mono {A B} : forall (D1 D2 : P (Comp (vfin A))) (K1 K2 : P A -> P (Comp B)),
+  D1 ⊆ D2 -> (forall x, K1 x ⊆ K2 x) ->
+  BIND D1 K1 ⊆ BIND D2 K2.
+Proof. 
+  intros D1 D2 K1 K2 subD subK.
+  unfold BIND.
+  move=> x [s1 [k1 [-> [inS1 inK1]]]]. 
+  exists s1. exists k1.
+  repeat split; auto.
+  specialize (subD _ inS1).
+  intros a aIn.
+  eapply subK.
+  eapply inK1.
+  auto.
+Qed.
+
+Lemma BIND_cong {A B} : forall (D1 D2 : P (Comp (vfin A))) (K1 K2 : P A -> P (Comp B)),
+  D1 ≃ D2 -> (forall x, K1 x ≃ K2 x) ->
+  BIND D1 K1 ≃ BIND D2 K2.
+Proof.
+intros D1 D2 K1 K2 [h1 h2] E2.
+split; eapply BIND_mono; eauto; intro x; destruct (E2 x); eauto.
+Qed.
+
+#[export] Instance Proper_Included_BIND {A B} : 
+  Proper (Included ==> (Logic.eq ==> Included) ==> Included) (@BIND A B).
+intros x1 y1 E1 x2 y2 E2. 
+eapply BIND_mono; eauto. 
+Qed. 
+
+#[export] Instance Proper_Same_BIND {A B} : Proper (Same_set ==> (Logic.eq ==> Same_set) ==> Same_set) (@BIND A B).
+unfold Proper. intros x1 y1 E1 x2 y2 E2.
+unfold respectful in E2.
+eapply BIND_cong; eauto.
+Qed.
+
+(* ------ Computation law ---- BIND (RETURN x) k = k x ------------------- *)
+
+Lemma bind_ret_Comp : forall {A B} (x : A) (k : A -> Comp B), 
+    bind (ret x) k = k x.
+Proof.
+  intros.
+  cbv.
+  destruct (k x); auto.
+  f_equal.
+  eapply app_nil_r.
+Qed. 
+
+Lemma BIND_RET1 : forall {A B} (x : P A) (k : P A -> P (Comp (vfin B))), 
+    monotone k ->  
+    BIND (RET x) k ⊆ k x.
+Proof.
+  intros A B x k MK. 
+  unfold BIND, RET.
+  repeat split.
+  intros y.
+  move =>[U [k0 [h2 [h3 h4]]]]. 
+  subst.
+  destruct U; try done.
+  destruct l; try done.
+  destruct l; try done.
+  cbn.
+  specialize (h4 v ltac:(cbv;eauto)).
+  rewrite append_Comp_nil.
+  eapply MK; eauto.
+Qed.
+
+Lemma BIND_RET2 : forall {A}{B} (x : P A) (k : P A -> P (Comp (vfin B))), 
+    monotone k -> 
+    continuous k ->
+    valid x ->
+    k x ⊆ BIND (RET x) k.
+Proof. 
+  intros A B x k km kc vx.
+  unfold continuous in kc. 
+  unfold BIND, RET.
+  intros y yIn.
+  unfold Ensembles.In.
+  have M: mem (y :: nil) ⊆ k x. intros z zIn.
+  { destruct zIn; try done. subst. auto. }
+  move: (kc _ vx (y :: nil) M) => [D [S1 S2]].
+  exists (c_multi (D :: nil)).
+  exists (fun _ => y).
+  repeat split; auto.
+  - cbn.
+    destruct y; auto. 
+    cbn. rewrite app_nil_r. auto.
+  - intros v vIn.
+    simpl in vIn. destruct vIn; try done.
+    subst.
+    eapply S2.
+    eauto.
+Qed.
+  
+Lemma BIND_RET : forall {A}{B} (x : P A) (k : P A -> P (Comp (vfin B))), 
+    monotone k -> 
+    continuous k ->
+    valid x ->
+    BIND (RET x) k ≃ k x.
+Proof.
+  intros.
+  split.
+  eapply BIND_RET1; eauto.
+  eapply BIND_RET2; eauto.
+Qed.
+
+(* ------------------------------------------------------------- *)
+(* monad law (right identity) *)
+
+Lemma monad_law {A} {y : Comp A} : y = x <- y;; ret x.
+Proof.
+  destruct y.
+  cbn. done.
+  cbn. 
+Admitted.
+
+Lemma RET_BIND2 : forall {A B} (m : P (Comp (vfin A))) (k : P A -> P (Comp (vfin B))), 
+    m ⊆ BIND m RET.
+Proof.
+  intros.
+  unfold BIND, RET.
+  intros y yIn.
+  unfold Ensembles.In.
+  exists y. exists ret.
+  repeat split; auto.
+  eapply monad_law.
+  intros V inV.
+  simpl. reflexivity.  
+Qed.
+
+(* NOTE: the opposite version is not true.
+
+   BIND m RET may contain some a in c_multi l that is a less precise
+   approximation of m. 
+*)
+
+Lemma RET_BIND1 : forall {A B} (m : P (Comp (vfin A))) (k : P A -> P (Comp (vfin B))), 
+    BIND m RET ⊆ m.
+Proof.
+  intros.
+  unfold BIND, RET.
+  intros y yIn.
+  unfold Ensembles.In in yIn.
+  move: yIn => [u1 [k1 [h1 [h2 h3]]]].
+  destruct u1; cbn in h2.
+  + subst. eauto.
+  + subst.
+    move: h2 h3.
+    induction l; intros h2 h3.
+    ++ cbn. auto.
+    ++ specialize (h3 a ltac:(simpl; auto)).
+       destruct (k1 a) eqn:h. done.
+       destruct l0; try done. destruct l0; try done.
+Abort.
+
+
+(* -------------------------------------------------------- *)
+(* Associative law *)
+
+   (* (m >>= g) >>= h = m >>= (\x -> g x >>= h) *)
+
+Lemma monad_associative_law {A}{B}{C}
+  {m : Comp A}{g : A -> Comp B}{h : B -> Comp C} : 
+  bind (bind m g) h = bind m (fun x => bind (g x) h).
+Admitted.
+
+
+Lemma BIND_ASSOC1 {A}{B}{C}
+  {m : P (Comp (vfin A))}
+  {g : P A -> P (Comp (vfin B)) }
+  {h : P B -> P (Comp (vfin C)) } : 
+   monotone g -> 
+   continuous g ->
+  BIND (BIND m g) h ⊆ BIND m (fun x => BIND (g x) h).  
+Proof.  
+  intros monoG contG.
+  unfold BIND.
+  intros x [s1 [k1 [-> [h1 h2]]]].
+  move: h1 => [s2 [k2 [-> [h3 h4]]]].
+  rewrite monad_associative_law.
+  exists s2. exists (fun x => y <- k2 x ;; k1 y). split. 
+  auto.
+  repeat split; auto.
+  intros v vin.
+  specialize (h4 v vin).
+  exists (k2 v). exists k1. 
+  repeat split; auto.
+  intros v2 v2in.
+  specialize (h2 v2).
+  eapply h2. 
+Abort. (* cannot make any more progress here. *)
+
+Lemma BIND_ASSOC2 {A}{B}{C}
+  {m : P (Comp (vfin A))}
+  {g : P A -> P (Comp (vfin B)) }
+  {h : P B -> P (Comp (vfin C)) } : 
+  BIND m (fun x => BIND (g x) h) ⊆ BIND (BIND m g) h.
+Proof.
+  unfold BIND.
+  intros x [s1 [k1 [-> [h1 h2]]]].
+  eexists. eexists.
+  repeat split.
+Abort. (* This seems even less likely to be true. *)  
+
+
+(* ---------------------------------------------------- *)
+
+Section Env.
+
+Context {Value : Type}.
+Let Rho := Env (P Value).
+
+Import EnvNotations.
+
+Lemma RET_continuous_env {D: Rho -> (P Value)}{ρ} : 
+  valid_env ρ ->
+  continuous_env D ρ ->
+  monotone_env D ->
+  continuous_env (fun ρ => RET (D ρ)) ρ.
+Proof.
+  intros VE IHD mD.
+  intros c cIn.
+  destruct c; try done.
+  destruct l; try done.
+  destruct l; try done.
+  destruct v.
+  cbn in cIn. 
+  have lemma: (exists ρ', exists _ : finite_env ρ', ρ' ⊆e ρ /\ ((mem x) ⊆ D ρ')).
+  { 
+    eapply continuous_In_sub; eauto.
+  }
+  destruct lemma as [ρ' [F' [S' h]]]. 
+  exists ρ'. exists F'.
+  split; auto.
+Qed.  
+
+Lemma BIND_continuous_env {A B} 
+  {D : Rho -> P (Comp (vfin A))} 
+  {K : Rho -> P A -> P (Comp B)} {ρ}: 
+  valid_env ρ -> 
+  continuous_env D ρ ->
+  monotone_env D ->
+  (forall v, continuous_env (fun ρ => K ρ v) ρ) ->
+  (forall v, monotone_env (fun ρ => K ρ v)) ->
+  continuous_env (fun ρ => (BIND (D ρ) (K ρ))) ρ. 
+Proof.
+  intros NE IHD mD IHK mK.
+  intros c cIn.
+  destruct cIn as [u [k [-> [uIn h2]]]].
+  destruct (IHD u uIn) as [ ρ1 [F1 [S1 uIn1]]].
+  destruct u.
+  + exists ρ1. exists F1. split; auto.
+    cbn. unfold BIND.
+    exists c_wrong. exists k.
+    repeat split. eapply uIn1.
+    intros a aIn. inversion aIn.
+  + have lemma :
+      forall l, 
+         (forall a : vfin A, Comp_In a (c_multi l) -> K ρ (vmem a) (k a)) -> 
+         exists ρ', exists (_ : finite_env ρ'), 
+           ρ' ⊆e ρ /\
+           (forall a : vfin A, Comp_In a (c_multi l) -> K ρ' (vmem a) (k a)).
+    { clear uIn ρ1 F1 S1 uIn1 l h2.
+      induction l; intros h2.
+      ++ exists (initial_finite_env ρ NE). eexists; repeat split; eauto.
+         intros a inA. simpl in inA. done.
+      ++ destruct IHl 
+          as [ρ2 [F2 [S2 uIn2]]].
+          { intros x xIn. apply h2. simpl. simpl in xIn. right.  auto. }
+          move: (h2 a ltac:(econstructor; eauto)) => Ka.
+          destruct (IHK (vmem a) _ Ka) as
+            [ρ1 [F1 [S1 uIn1]]].
+          have SS1: same_scope ρ1 ρ. eapply Forall2_same_scope; eauto.
+          have SS2: same_scope ρ2 ρ. eapply Forall2_same_scope; eauto.
+          have SS: same_scope ρ1 ρ2. { transitivity ρ; auto. symmetry; auto. }
+          exists (ρ1 ⊔e ρ2).
+          repeat split.
+          - eapply join_finite_env; eauto.    
+          - eapply join_lub; eauto.
+          - intros x xIn. simpl in xIn. destruct xIn. 
+            subst. eapply (mK (vmem x)); try eassumption. eapply join_sub_left; auto.
+            eapply (mK (vmem x)). 2: { eapply uIn2; eauto. }
+            eapply join_sub_right; eauto.
+    }
+    destruct (lemma l h2) as 
+      [ρ2 [F2 [S2 In2]]]. clear lemma.
+    have SS1: same_scope ρ1 ρ. eapply Forall2_same_scope; eauto.
+    have SS2: same_scope ρ2 ρ. eapply Forall2_same_scope; eauto.
+    have SS: same_scope ρ1 ρ2. { transitivity ρ; auto. symmetry; auto. }
+    exists (ρ1 ⊔e ρ2).
+    repeat split.
+    - eapply join_finite_env; eauto.    
+    - eapply join_lub; eauto.
+    - exists (c_multi l). exists k.
+    repeat split; eauto.
+    eapply mD; try eassumption. eapply join_sub_left; auto.
+    intros a aIn.
+    eapply (mK (vmem a)). 2: { eapply In2; eauto. }
+    eapply join_sub_right; eauto.
+Qed.                 
+
+End Env.
+
+(* ----------------------------------------------------------------------- *)
+
+Lemma BIND_monotone {Value A B} 
+  {D : P Value -> P (Comp (vfin A))} 
+  {K : P Value -> P A -> P (Comp B)}: 
+  monotone D ->
+  (forall v, monotone (fun x => K x v)) ->
+  monotone (fun v => (BIND (D v) (K v))). 
+Proof. 
+  intros mD mK x y S.
+  eapply BIND_mono; eauto. 
+  intro z; eapply mK; auto.
+Qed.
+ 
+Lemma BIND_continuous {Value A B} 
+  {D : P Value -> P (Comp (vfin A))} 
+  {K : P Value -> P A -> P (Comp B)}: 
+  continuous D ->
+  monotone D ->
+  (forall v, continuous (fun x => K x v)) ->
+  (forall v, monotone (fun x => K x v)) ->
+  continuous (fun v => (BIND (D v) (K v))). 
+Proof.
+  intros IHD mD IHK mK.
+  intros w VW F SUB.
+  induction F.
+  - destruct VW as [v vIn].
+    have VW : valid w. econstructor; eauto.
+    destruct (IHD w VW nil ltac:(cbv; done)) as [D1 [IS1 OS1]]. 
+    exists D1.
+    repeat split; eauto.
+    cbv. done.
+  - destruct IHF as [D1 [IS1 OS1]]. 
+    intros y yIn. eapply SUB. right. auto.
+    have C: a ∈ BIND (D w)(K w). eapply SUB. left.  auto.
+    destruct C as [u [k [uIn [h1 h2]]]].    
+    unfold continuous in IHD.
+    destruct (IHD w VW (u :: nil) ltac:(eauto)) as [D2 [IS2 OS2]]. 
+    destruct u.
+    + simpl in h1. subst.
+      exists (vfin_Union D1 D2).
+      repeat rewrite vmem_Union.
+      repeat split; eauto.
+      eapply union_left; auto.
+      cbn.
+      intros z zIn. 
+      destruct zIn; subst.
+      ++ exists c_wrong. exists k.
+         repeat split.
+         eapply mD. 2: eapply OS2; auto.
+         auto.
+         intros x h. inversion h.
+      ++ specialize (OS1 z H).
+         eapply BIND_mono.
+         3: eapply OS1.
+         eapply mD. auto.
+         intros x y yIn.
+         eapply mK. 2: eapply yIn. auto.
+    + have lemma:          
+      forall l, 
+         (forall a : vfin A, Comp_In a (c_multi l) -> K w (vmem a) (k a)) -> 
+         exists D0, (vmem D0 ⊆ w) /\
+           (forall a : vfin A, Comp_In a (c_multi l) -> K (vmem D0) (vmem a) (k a)).
+      { clear uIn D1 IS1 OS1 OS2 h1 h2.
+        induction l0; intros h2.
+        ++ exists D2. 
+           repeat split; eauto.
+           intros a0 a0In.
+           simpl in a0In. done.
+        ++ destruct IHl0 as [D3 [IS3 OS3]].
+           { intros x xIn. apply h2. simpl. simpl in xIn. right. auto. }
+           move: (h2 a0 ltac:(econstructor; eauto)) => Ka.
+           specialize (IHK (vmem a0) w VW (k a0 :: nil)) as [D4 [IS4 OS4]].
+           { rewrite <- In_Sub. auto. }
+           exists (vfin_Union D3 D4).
+           repeat rewrite vmem_Union.
+           repeat split; eauto.
+           eapply union_left; auto. 
+           intros y yIn. destruct yIn.  
+           subst. eapply mK. 2: eapply OS4. eapply sub_union_right. eauto.
+           eapply mK. 2: eapply OS3. eapply sub_union_left. eauto.
+      }
+      destruct (lemma l h2) as [D3 [IS3 OS3]].
+      exists (vfin_Union D1 (vfin_Union D2 D3)).
+      repeat rewrite vmem_Union.
+      repeat split; eauto.
+      eapply union_left; auto.  eapply union_left; auto.
+      intros y yIn. destruct yIn.
+      ++ subst a. subst y.
+         exists (c_multi l). exists k.
+         repeat split; eauto.
+         eapply mD. 2: eapply OS2; eauto. right. left. auto.
+         intros x xIn.
+         eapply mK. 2: eapply OS3; eauto.
+         right. right. auto.
+      ++ eapply BIND_mono. 3: eapply OS1; auto.
+         eapply mD. left. auto.
+         intros v z zIn. eapply mK. 2: eapply zIn. left. auto.
+Qed.
+
+Lemma RET_monotone  {Value A} {D : P Value -> P A } :
+  monotone D -> monotone (fun v : P Value => RET (D v)).
+Proof. intros mD x y S. eapply RET_mono; eauto. Qed.
+
+
+Lemma RET_continuous {Value A} {D : P Value -> P A } :
+  continuous D -> monotone D -> continuous (fun v : P Value => RET (D v)).
+Proof.
+  intros IHD mD.
+  intros w VW F SUB.
+  induction F.
+  - destruct (IHD w VW nil ltac:(cbv; done)) as [D1 [IS1 OS1]].
+    exists D1.
+    repeat split; eauto.
+    cbv. done.
+  - destruct IHF as [D1 [IS1 OS1]].
+    intros y yIn. eapply SUB. right. auto.
+    have C: a ∈ RET (D w). eapply SUB. left.  auto.
+    destruct a; try done.
+    destruct l; try done.
+    destruct l; try done.
+    cbn in C.
+    unfold continuous in IHD.
+    destruct v as [l NE]. simpl in C.
+    destruct (IHD w VW l ltac:(eauto)) as [D2 [IS2 OS2]].
+    exists (vfin_Union D1 D2).
+    rewrite vmem_Union.
+    repeat split; eauto.
+    eapply union_left; eauto.
+    intros y yIn. 
+    destruct yIn.
+    ++ subst.
+       cbn. intros z zIn. specialize (OS2 z zIn). 
+       eapply mD. 2: eapply OS2. eauto.
+    ++ specialize (OS1 y H).
+       eapply RET_mono. 2: eapply OS1. auto.
+Qed.
+
+
