coq/denot/semantic_notions.v
@@ -1,0 +1,411 @@
+Require Import Coq.Logic.FunctionalExtensionality.
+Require Import Coq.Classes.RelationClasses.
+Require Coq.Relations.Relation_Definitions.
+Require Import Lia.
+
+Require Export lc.tactics.
+Require Import structures.Structures.
+
+Import MonadNotation.
+Open Scope monad_scope.
+Import SetNotations.
+Local Open Scope set_scope.
+
+(* ------------------------------------------------------- *)
+(* More Set stuff *)
+
+(* Sets (could be infinite)    P A  == A -> Prop           *)
+(* Nonempty Sets               { X : P A | valid X }       *)
+(* Finite sets                 list A                      *)
+(* Nonempty finite sets        { X : list A | X <> nil }   *)
+(* coercion                    mem : list A -> P A         *)
+
+(* ------------------------------------------------------- *)
+
+
+Definition vfin (A : Type) : Type := { X : list A | X <> nil }. 
+Definition vmem {A : Type} : vfin A -> P A := fun '(exist _ X _) => mem X.
+
+Definition finite {A} (X : P A) : Prop := exists E, (X ≃ mem E).
+Definition vfinite {A} (X : P A) : Prop := exists E, (X ≃ vmem E).
+
+(* deprecate *)
+Definition valid {A : Type } (V : P A) : Type := nonemptyT V.
+Definition valid_mem {A : Type} (V : list A) : Prop := V <> nil.
+
+
+
+Definition vfin_Singleton {A : Type } : A -> vfin A.
+intro x. exists (x :: nil). intro h.  done. Defined.
+
+Definition vfin_Union {A : Type} : vfin A -> vfin A -> vfin A.
+intros [X NEX] [Y NEY]. exists (X ++ Y). destruct X; try done. Defined.
+
+Lemma vmem_Singleton {A:Type}{x : A} :
+  vmem (vfin_Singleton x) ≃ ⌈ x ⌉.
+Proof.
+  cbn. eapply mem_singleton_eq. 
+Qed.
+
+Lemma vmem_Union {A:Type}{D1 D2 : vfin A} :
+  vmem (vfin_Union D1 D2) = (vmem D1 ∪ vmem D2).
+Proof.
+  destruct D1. destruct D2.
+  cbn.
+  eapply union_mem.
+Qed.
+
+
+Lemma finite_singleton : forall {B} (v : B), vfinite ⌈ v ⌉.
+Proof. intros B v.  
+       have NE: (cons v nil) <> nil. done.
+       exists (exist _ (cons v nil) NE).
+       cbn. rewrite mem_singleton_eq. reflexivity. 
+Qed.
+
+Lemma vfinite_Union {A : Type} : forall (X : P A), vfinite X -> forall Y, vfinite Y -> vfinite (X ∪ Y).
+Proof.
+  intros X [fX eX] Y [fY eY].
+  exists (vfin_Union fX fY).
+  destruct fX as [x n].
+  destruct fY as [y m].
+  cbn. cbn in eX. cbn in eY.
+  rewrite union_mem.
+  rewrite eX. rewrite eY.
+  reflexivity.
+Qed.
+
+
+Lemma union_left {A}{X Y Z: P A} : X ⊆ Z -> Y ⊆ Z -> X ∪ Y ⊆ Z.
+Proof. intros h1 h2.
+       intros x xIn. destruct xIn; eauto.
+Qed.
+
+
+#[export] Hint Resolve finite_singleton vfinite_Union : core.
+
+
+Lemma In_mem_Included {A}{d:A}{D} : 
+    d ∈ D ->
+    mem (d :: nil) ⊆ D.
+Proof.
+  intros.
+  intros y yIn. destruct yIn. subst; auto. done.
+Qed.
+
+Lemma Included_mem_In {A}{d:A}{D} : 
+    mem (d :: nil) ⊆ D ->
+    d ∈ D.
+
+Proof.
+  intros.
+  specialize (H d). eapply H. eauto.
+Qed.
+
+Lemma mem_app_Included {A}{D1 D2 : list A}{w} : 
+ mem D1 ⊆ w ->
+ mem D2 ⊆ w ->
+ mem (D1 ++ D2) ⊆ w.
+Proof. 
+  intros.
+  rewrite union_mem. intros y yIn. induction yIn; eauto.
+Qed.
+
+Lemma mem_app_valid {A}{D1 D2 : list A}: 
+  valid_mem D1 ->
+  valid_mem D2 ->
+  valid_mem (D1 ++ D2).
+Proof. intros.
+ unfold valid_mem in *. destruct D1; try done.
+Qed.
+
+#[export] Hint Resolve In_mem_Included Included_mem_In mem_app_Included mem_app_valid : core.
+
+
+(* ------------------------------------------------------- *)
+(* These definitions are independent of a given value type type *)
+
+
+Definition monotone {A}{B} (F : P A -> P B) : Set := 
+  forall D1 D2, (D1 ⊆ D2) -> F D1 ⊆ F D2.
+
+(* aka sub_preserving *)
+Definition sub_reflecting {A}{B} (F : P A -> P B) : Set := 
+  forall D1 D2, F D1 ⊆ F D2 -> (D1 ⊆ D2).
+
+(* Note: mem E could be empty *)
+Definition continuous {A}{B} (F : P A -> P B) : Set :=
+  forall (X : P A), valid X ->
+               forall E, mem E ⊆ F X ->
+                    exists D, (vmem D ⊆ X) /\ ((mem E) ⊆ F (vmem D)).
+
+
+(* ------------------------------------------------------- *)
+
+
+Module EnvNotations.
+Notation "ρ ⋅ x" := (Env.access (fun x => False) ρ x) (at level 50).
+Infix "⊔e" := (Env.map2 Union) (at level 60).
+Infix "⊆e" := (Env.Forall2 Included) (at level 50).
+End EnvNotations.
+Import EnvNotations.
+
+
+Section EnvDefinitions.
+
+Context {Value : Type}.
+Let Rho := Env (P Value).
+
+Definition monotone_env {A} (D : Rho -> P A) := 
+  forall ρ ρ' , ρ ⊆e ρ' -> (D ρ) ⊆ D ρ'.
+
+Definition nonempty_env : Rho -> Type := Env.ForallT nonemptyT.
+
+Definition valid_env : Rho -> Type := Env.ForallT valid. 
+
+Definition sub_env : Rho -> Rho -> Prop := Env.Forall2 Included.
+
+Definition same_env : Rho -> Rho -> Prop := Env.Forall2 Same_set.
+
+Definition finite_env : Rho -> Type := Env.ForallT vfinite.
+
+Definition continuous_In {A} (D:Rho -> P A) (ρ:Rho) (v:A) : Prop :=
+  v ∈ D ρ -> exists ρ' , exists (pf : finite_env ρ'),  ρ' ⊆e ρ /\ (v ∈ D ρ').
+
+Definition continuous_env {A} (D:Rho -> P A) (ρ:Rho) : Prop :=
+  forall (v : A), continuous_In D ρ v.
+
+Definition continuous_Sub {A} (D:Rho -> P A) (ρ:Rho) (V:list A) : Prop :=
+  mem V ⊆ D ρ -> 
+  exists ρ', exists (pf : finite_env ρ'),
+    ρ' ⊆e ρ  /\ (mem V ⊆ D ρ').
+
+(* ----------------------------------------------------- *)
+
+(* Join environments *)
+
+Lemma join_finite_env {ρ1 ρ2} : 
+  same_scope ρ1 ρ2 
+  -> finite_env ρ1
+  -> finite_env ρ2
+  -> finite_env (ρ1 ⊔e ρ2).
+Proof.
+  move: ρ2.
+  induction ρ1 as [|[x1 v1] r1].
+  all: intros ρ2 sc h1; destruct ρ2 as [|[x2 v2] r2]; intros h2; simpl; eauto.
+  inversion h1; subst; clear h1.
+  inversion h2; subst; clear h2.
+  destruct (x1 == x2); subst.
+  + econstructor; eauto. eapply IHr1; eauto. inversion sc. auto.
+    rewrite sub_dom1; auto.
+  + assert False. inversion sc. subst. done. done.
+Qed.
+
+Lemma join_lub {ρ ρ1 : Rho} :
+  same_scope ρ1 ρ ->
+  forall ρ2, same_scope ρ2 ρ ->
+  ρ1 ⊆e ρ -> ρ2 ⊆e ρ -> (ρ1 ⊔e ρ2) ⊆e ρ.
+Proof.
+  intro SS1.
+  induction SS1; intros ρ2 SS2; inversion SS2; subst.
+  simpl. auto.
+  intros.
+  simpl.
+  inversion H1. inversion H2. subst.
+  rewrite eq_dec_refl.
+  eapply Env.Forall2_cons; eauto.
+  rewrite sub_dom1. auto.
+  rewrite -> H21.
+  rewrite -> H13.
+  rewrite union_idem.
+  reflexivity.
+Qed.
+  
+Lemma join_sub_left {ρ1 ρ2 : Rho} : 
+  same_scope ρ1 ρ2 ->
+  ρ1 ⊆e (ρ1 ⊔e ρ2).
+Proof.
+  intros h.
+  induction h; simpl; eauto.
+  rewrite eq_dec_refl.
+  econstructor; eauto. 
+Qed.
+
+Lemma join_sub_right {ρ1 ρ2 : Rho} : 
+  same_scope ρ1 ρ2 ->
+  ρ2 ⊆e (ρ1 ⊔e ρ2).
+Proof.
+  induction 1; simpl; eauto. 
+  rewrite eq_dec_refl.
+  econstructor; eauto. 
+  erewrite Forall2_dom in H0; eauto.
+Qed.
+
+(* --------------------------------------- *)
+
+(* Initial environment. *)
+
+(* creates an environment that maps each variable x to a singleton 
+   set of some element in ρ x *)
+Definition initial_finite_env (ρ : Rho) (NE : valid_env ρ) : Rho.
+  induction NE. exact nil.
+  destruct f as [V _].
+  exact (cons (x, ⌈ V ⌉) IHNE).
+Defined.
+
+Lemma initial_finite_dom : forall E NE, dom (initial_finite_env E NE) = dom E.
+Proof.
+  induction NE; simpl. auto.
+  destruct f as [v w].  simpl. congruence.
+Qed. 
+
+Lemma initial_fin (ρ : Rho) (NE : valid_env ρ) :
+  finite_env (initial_finite_env ρ NE).
+Proof.
+  induction NE.
+  simpl. econstructor.
+  simpl. destruct f as [v w1 ].
+  econstructor; eauto.
+  rewrite initial_finite_dom. auto.
+Qed.
+
+Lemma initial_fin_sub (ρ : Rho) (NE : valid_env ρ) :
+  initial_finite_env ρ NE ⊆e ρ.
+Proof.
+  induction NE; simpl. econstructor.
+  destruct f as [v fx].
+  econstructor. auto.
+  rewrite initial_finite_dom. auto.
+  intros z y. inversion y. subst. unfold In. auto.
+Qed.
+
+(* single-env maps x to D and any other variable y to something in ρ y. *)
+Definition single_env (x : atom) (D : P Value) (ρ : Rho) 
+  (NE : valid_env ρ) : Rho :=
+  update x D (initial_finite_env ρ NE).
+
+  
+Lemma single_fin { X x ρ NE } : 
+  vfinite X ->
+  finite_env (single_env x X ρ NE).
+Proof.
+  induction NE; intro FIN; unfold finite_env; eauto.
+  unfold single_env; econstructor.
+  unfold single_env. simpl. 
+  destruct f as [v1 v2].
+  destruct (x == x0) eqn:EQ.
+  + subst. rewrite update_eq_var. 
+    econstructor.
+    eapply initial_fin. 
+    rewrite initial_finite_dom.
+    auto. 
+    auto.
+  + rewrite update_neq_var; eauto.
+    econstructor; eauto.
+    eapply IHNE; eauto.
+    Search dom update.
+    rewrite dom_update.
+    rewrite initial_finite_dom.
+    auto.
+Qed.
+
+Lemma single_sub { ρ : Rho }{ x V } :
+  forall (NE : valid_env ρ),
+    V ⊆ (ρ ⋅ x)
+  -> x `in` dom ρ
+  -> (single_env x V ρ NE) ⊆e ρ.
+Proof.
+  intros NE.
+  induction NE.
+  all: intros vpe Indom. 
+  + (* nil case *) cbn. auto. 
+  + (* cons case *)
+    unfold single_env in *.
+    simpl. simpl_env in Indom.
+    destruct f as [w h2]. simpl.
+    simpl in vpe.
+    destruct (x == x0).
+    ++ subst. econstructor; eauto.
+       eapply initial_fin_sub.
+       rewrite initial_finite_dom. 
+       eauto.
+    ++ econstructor; eauto. 
+       eapply IHNE; eauto. fsetdec.
+       simpl_env. 
+       rewrite initial_finite_dom. auto.
+       intros h hIn. inversion hIn. subst. auto.
+Qed.
+
+Lemma update_access : forall {x ρ NE X},
+  x `in` dom ρ ->
+  X ≃ (single_env x X ρ NE) ⋅ x.
+Proof.
+  intros.
+  unfold single_env.
+  move: NE.
+  induction NE. fsetdec.
+  simpl. destruct f as [w h2]. simpl.
+  destruct (x == x0) eqn:EQ. subst. simpl.
+  rewrite eq_dec_refl. reflexivity.
+  simpl. rewrite EQ. eapply IHNE; auto. simpl in H. fsetdec.
+Qed.  
+
+(* v∈single[xv]x  *)
+Lemma v_single_xvx {v x ρ NE} : 
+  x `in` dom ρ ->
+  v ∈ (single_env x ⌈ v ⌉ ρ NE ⋅ x).
+Proof.
+  unfold single_env.
+  move: NE.
+  induction NE; intro h. fsetdec.
+  simpl. destruct f as [w h2]. simpl.
+  destruct (x == x0) eqn:EQ. subst. simpl.
+  rewrite eq_dec_refl. econstructor; eauto.
+  simpl. rewrite EQ. simpl in h. eapply IHNE; auto. fsetdec.
+Qed.  
+
+
+(* --------------------------------------- *)
+(* continuous-∈⇒⊆ *)
+
+Lemma continuous_In_sub {A} (E : Rho -> (P A)) ρ (NE : valid_env ρ) :
+   monotone_env E
+   -> forall V, mem V ⊆ E ρ
+   -> (forall v, v ∈ mem V -> continuous_In E ρ v)
+   -> exists ρ', exists (pf : finite_env ρ') ,  ρ' ⊆e ρ /\ (mem V ⊆ E ρ').
+Proof.
+  intros me VS VE vcont.
+  induction VS.
+  - exists (initial_finite_env ρ NE).
+    repeat split.
+    eapply (initial_fin ρ NE).
+    eapply initial_fin_sub; eauto. 
+    done.
+  - destruct IHVS as [ ρ1 [ fρ1 [ ρ1ρ VEρ1 ]]].
+    intros d z. eapply VE; eauto.
+    intros v VM. eapply vcont; eauto.
+    destruct (vcont a) as [ρ2 [fρ2 [ρ2ρ VEρ2]]].
+    econstructor; eauto.
+    eapply VE. econstructor; eauto.
+    exists (ρ1 ⊔e ρ2).
+    have S1: same_scope ρ1 ρ. eapply Forall2_same_scope; eauto.
+    have S2: same_scope ρ2 ρ. eapply Forall2_same_scope; eauto. 
+    have SS: same_scope ρ1 ρ2. 
+    { transitivity ρ; auto. symmetry; auto. }
+    eexists. eapply join_finite_env; eauto.
+    repeat split.
+    + eapply join_lub; eauto.
+    + intros d dm.
+    inversion dm; subst.
+    eapply me. eapply join_sub_right; eauto. auto. 
+    eapply me. eapply join_sub_left; eauto. auto.
+Qed.
+
+End EnvDefinitions.
+
+#[export] Hint Resolve finite_singleton : core. 
+#[export] Hint Resolve initial_fin : core. 
+#[export] Hint Resolve initial_fin_sub : core. 
+#[export] Hint Resolve single_fin : core. 
+#[export] Hint Resolve single_sub : core. 
+#[export] Hint Resolve v_single_xvx : core. 
